2D eq-point example in the 2-index style RST effect

examples/lowstar_resources/EqPoint.TwoIndex.fst
@@ -13,7 +13,7 @@
    See the License for the specific language governing permissions and
    limitations under the License.
 *)
-module Point.TwoIndex
+module EqPoint.TwoIndex
 
 open FStar.HyperStack.ST
 module B = LowStar.Buffer
@@ -29,22 +29,23 @@ open LowStar.BufferOps
 
 abstract
 noeq
-type point = {
+type eq_point = {
     x: B.pointer int;
     y: B.pointer int
   }
 
-type point_view_t = {
+type eq_point_view_t = {
     x_view: int;
-    y_view: int
+    y_view: y_view:int{x_view = y_view}
   }
 
 abstract
-let point_view (p:point) : view point_view_t = 
+let eq_point_view (p:eq_point) : view eq_point_view_t = 
   let fp = Ghost.hide (B.loc_union (B.loc_addr_of_buffer p.x) (B.loc_addr_of_buffer p.y)) in
   let inv h = 
     B.live h p.x /\ B.live h p.y /\ B.freeable p.x /\ B.freeable p.y /\ 
-    B.loc_disjoint (B.loc_addr_of_buffer p.x) (B.loc_addr_of_buffer p.y) 
+    B.loc_disjoint (B.loc_addr_of_buffer p.x) (B.loc_addr_of_buffer p.y) /\
+    Seq.index (B.as_seq h p.x) 0 == Seq.index (B.as_seq h p.y) 0 
   in
   let sel (h:imem inv) = 
     { 
@@ -59,29 +60,32 @@ let point_view (p:point) : view point_view_t =
     sel = sel
   }
 
-let point_resource (p:point) = 
-  as_resource (point_view p)
+let eq_point_resource (p:eq_point) = 
+  as_resource (eq_point_view p)
 
-let sel_x (p:point) (h:imem (inv (point_resource p))) : GTot int = 
-  (sel (point_view p) h).x_view
+let sel_x (p:eq_point) (h:imem (inv (eq_point_resource p))) : GTot int = 
+  (sel (eq_point_view p) h).x_view
   
-let sel_y (p:point) (h:imem (inv (point_resource p))) : GTot int = 
-  (sel (point_view p) h).y_view
+let sel_y (p:eq_point) (h:imem (inv (eq_point_resource p))) : GTot int = 
+  (sel (eq_point_view p) h).y_view
 
-let mk_point (x y:B.pointer int) : point = 
+let mk_eq_point (x y:B.pointer int) 
+  : Pure eq_point (requires (B.loc_disjoint (B.loc_buffer x) (B.loc_buffer y)))
+                  (ensures (fun _ -> True)) = 
   {
     x = x;
     y = y
   }
 
-let unpack (p:point)
+let unpack (p:eq_point)
   : RST (B.pointer int & B.pointer int) 
-        (point_resource p)
+        (eq_point_resource p)
         (fun (x,y) -> ptr_resource x <*> ptr_resource y)
         (fun _ -> True)
         (fun h0 (x,y) h1 -> 
           sel_x p h0 = sel (ptr_view x) h1 /\ 
-          sel_y p h0 = sel (ptr_view y) h1) = 
+          sel_y p h0 = sel (ptr_view y) h1 /\
+          sel (ptr_view x) h1 = sel (ptr_view y) h1) = 
   reveal_star ();
   reveal_ptr ();
   reveal_rst_inv ();
@@ -89,10 +93,10 @@ let unpack (p:point)
   (p.x,p.y)
 
 let pack (x y:B.pointer int)
-  : RST point
+  : RST eq_point
         (ptr_resource x <*> ptr_resource y)
-        (fun p -> point_resource p)
-        (fun _ -> True)
+        (fun p -> eq_point_resource p)
+        (fun h -> sel (ptr_view x) h = sel (ptr_view y) h)
         (fun h0 p h1 -> 
           sel_x p h1 = sel (ptr_view x) h0 /\ 
           sel_y p h1 = sel (ptr_view y) h0) = 
@@ -100,14 +104,15 @@ let pack (x y:B.pointer int)
   reveal_ptr ();
   reveal_rst_inv ();
   reveal_modifies ();
-  mk_point x y
+  mk_eq_point x y
 
-let get_x (p:point)
-  : RST int (point_resource p)
-            (fun _ -> point_resource p)
+let get (p:eq_point)
+  : RST int (eq_point_resource p)
+            (fun _ -> eq_point_resource p)
             (fun _ -> True)
-            (fun h0 x h1 -> 
-               sel_x p h1 = x /\
+            (fun h0 xy h1 -> 
+               sel_x p h1 = xy /\
+               sel_y p h1 = xy /\
                sel_x p h1 = sel_x p h0 /\
                sel_y p h1 = sel_y p h0) = 
   reveal_star ();
@@ -119,91 +124,44 @@ let get_x (p:point)
             (ptr_resource p.y) 
             (fun _ -> ptr_read p.x)
 
-let get_y (p:point)
-  : RST int (point_resource p)
-            (fun _ -> point_resource p)
-            (fun _ -> True)
-            (fun h0 y h1 -> 
-               sel_x p h1 = sel_x p h0 /\
-               sel_y p h1 = sel_y p h0 /\
-               sel_y p h1 = y) = 
-  reveal_star ();
-  reveal_ptr ();
-  reveal_rst_inv ();
-  reveal_modifies ();
-  rst_frame #(ptr_resource p.x <*> ptr_resource p.y) #_ #_
-            #(fun _ -> ptr_resource p.x <*> ptr_resource p.y)
-            (ptr_resource p.x) 
-            (fun _ -> ptr_read p.y)
-
-let set_x (p:point) (x:int)
-  : RST unit (point_resource p)
-             (fun _ -> point_resource p)
+let move_up (p:eq_point)
+  : RST unit (eq_point_resource p)
+             (fun _ -> eq_point_resource p)
              (fun _ -> True)
-             (fun h0 _ h1 -> 
-                sel_x p h1 = x /\
-                sel_y p h1 = sel_y p h0) = 
+             (fun h0 _ h1 ->
+                sel_x p h1 = sel_x p h0 + 1 /\
+                sel_y p h1 = sel_y p h0 + 1) =
   reveal_star ();
   reveal_ptr ();
   reveal_rst_inv ();
   reveal_modifies ();
+  let xy = get p in 
   rst_frame #(ptr_resource p.x <*> ptr_resource p.y) #_ #_
             #(fun _ -> ptr_resource p.x <*> ptr_resource p.y)
             (ptr_resource p.y) 
-            (fun _ -> ptr_write p.x x)
+            (fun _ -> ptr_write p.x (xy + 1));
+  rst_frame #(ptr_resource p.x <*> ptr_resource p.y) #_ #_
+            #(fun _ -> ptr_resource p.x <*> ptr_resource p.y)
+            (ptr_resource p.x) 
+            (fun _ -> ptr_write p.y (xy + 1))
 
-let set_y (p:point) (y:int)
-  : RST unit (point_resource p)
-             (fun _ -> point_resource p)
+let move_down (p:eq_point)
+  : RST unit (eq_point_resource p)
+             (fun _ -> eq_point_resource p)
              (fun _ -> True)
-             (fun h0 _ h1 -> 
-                sel_x p h1 = sel_x p h0 /\
-                sel_y p h1 = y) = 
+             (fun h0 _ h1 ->
+                sel_x p h1 = sel_x p h0 - 1 /\
+                sel_y p h1 = sel_y p h0 - 1) =
   reveal_star ();
   reveal_ptr ();
   reveal_rst_inv ();
   reveal_modifies ();
+  let xy = get p in 
+  rst_frame #(ptr_resource p.x <*> ptr_resource p.y) #_ #_
+            #(fun _ -> ptr_resource p.x <*> ptr_resource p.y)
+            (ptr_resource p.y) 
+            (fun _ -> ptr_write p.x (xy - 1));
   rst_frame #(ptr_resource p.x <*> ptr_resource p.y) #_ #_
             #(fun _ -> ptr_resource p.x <*> ptr_resource p.y)
             (ptr_resource p.x) 
-            (fun _ -> ptr_write p.y y)
-
-let move_up (p:point)
-  : RST unit (point_resource p)
-             (fun _ -> point_resource p)
-             (fun _ -> True)
-             (fun h0 _ h1 -> 
-               sel_x p h1 = sel_x p h0 /\ 
-               sel_y p h1 = sel_y p h0 + 1) = 
-  let y = get_y p in
-  set_y p (y + 1)
-
-let move_down (p:point)
-  : RST unit (point_resource p)
-             (fun _ -> point_resource p)
-             (fun _ -> True)
-             (fun h0 _ h1 -> 
-               sel_x p h1 = sel_x p h0 /\ 
-               sel_y p h1 = sel_y p h0 - 1) = 
-  let y = get_y p in
-  set_y p (y - 1)
-
-let move_right (p:point)
-  : RST unit (point_resource p)
-             (fun _ -> point_resource p)
-             (fun _ -> True)
-             (fun h0 _ h1 -> 
-               sel_x p h1 = sel_x p h0 + 1 /\ 
-               sel_y p h1 = sel_y p h0) = 
-  let x = get_x p in
-  set_x p (x + 1)
-
-let move_left (p:point)
-  : RST unit (point_resource p)
-             (fun _ -> point_resource p)
-             (fun _ -> True)
-             (fun h0 _ h1 -> 
-               sel_x p h1 = sel_x p h0 - 1 /\ 
-               sel_y p h1 = sel_y p h0) = 
-  let x = get_x p in
-  set_x p (x - 1)
+            (fun _ -> ptr_write p.y (xy - 1))
